before change syntax

OperationalSemantics.v
@@ -16,39 +16,39 @@ Reserved Notation "α '⊧' t1 '↪{' β '}' t2" (at level 60, t1 constr, β con
 (* Because in this formalization, we treat pure operations as effectful
 operations, the rule [STPureOp] is not necessary. *)
 Inductive step : list evop -> tm -> list evop -> tm -> Prop :=
-| STEffOp: forall (α: list evop) op (c1 c: constant) e,
+| STEffOp: forall (α β: list evop) op (c1 c: constant) e,
     body e -> lc c1 -> lc c ->
-    α ⊧{ op ~ c1 }⇓{ c } ->
-    α ⊧ (tleteffop op c1 e) ↪{ [ev{ op ~ c1 := c}] } (e ^t^ c)
+    α ⊧{ op ~ c1 }⇓{ β }{ c } ->
+    α ⊧ (tleteffop op c1 e) ↪{ β } (e ^t^ c)
 | STLetE1: forall α β e1 e1' e,
     body e ->
     α ⊧ e1 ↪{β} e1' ->
     α ⊧ (tlete e1 e) ↪{β} (tlete e1' e)
 | STLetE2: forall α (v1: value) e,
     lc v1 -> body e ->
-    α ⊧ (tlete (treturn v1) e) ↪{ [] } (e ^t^ v1)
+    α ⊧ (tlete (treturn v1) e) ↪{ α } (e ^t^ v1)
 | STLetAppLam: forall α T (v_x: value) e1 e,
     body e1 -> body e -> lc v_x ->
-    α ⊧ (tletapp (vlam T e1) v_x e) ↪{ [] } tlete (e1 ^t^ v_x) e
+    α ⊧ (tletapp (vlam T e1) v_x e) ↪{ α } tlete (e1 ^t^ v_x) e
 | STLetAppFix: forall α T_f (v_x: value) (e1: tm) e,
     body (vlam T_f e1) -> lc v_x -> body e ->
-    α ⊧ tletapp (vfix T_f (vlam T_f e1)) v_x e ↪{ [] }
+    α ⊧ tletapp (vfix T_f (vlam T_f e1)) v_x e ↪{ α }
             tletapp ((vlam T_f e1) ^v^ v_x) (vfix T_f (vlam T_f e1)) e
 | STMatchbTrue: forall α e1 e2,
     lc e1 -> lc e2 ->
-    α ⊧ (tmatchb true e1 e2) ↪{ [] } e1
+    α ⊧ (tmatchb true e1 e2) ↪{ α } e1
 | STMatchbFalse: forall α e1 e2,
     lc e1 -> lc e2 ->
-    α ⊧ (tmatchb false e1 e2) ↪{ [] } e2
+    α ⊧ (tmatchb false e1 e2) ↪{ α } e2
 where "α '⊧' t1 '↪{' β '}' t2" := (step α t1 β t2).
-  
+
 Inductive multistep : list evop -> tm -> list evop -> tm -> Prop :=
 | multistep_refl : forall α (e : tm),
-    lc e -> multistep α e [] e
-| multistep_step : forall  α β β' (x y z: tm),
+    lc e -> multistep α e α e
+| multistep_step : forall  α β γ (x y z: tm),
     α ⊧ x ↪{ β } y ->
-    multistep (α ++ β) y β' z ->
-    multistep α x (β ++ β') z.
+    multistep β y γ z ->
+    multistep α x γ z.
 
 Notation "α '⊧' t1 '↪*{' β '}' t2" := (multistep α t1 β t2) (at level 60, t1 constr, β constr).
 
@@ -94,21 +94,16 @@ Global Hint Resolve step_regular2: core.
 Theorem multistep_trans :
   forall α βx βy (x y z : tm),
    α ⊧ x ↪*{ βx } y ->
-   (α ++ βx) ⊧ y ↪*{ βy } z ->
-   α ⊧ x ↪*{ βx ++ βy } z.
+   βx ⊧ y ↪*{ βy } z ->
+   α ⊧ x ↪*{ βy } z.
 Proof.
   intros. generalize dependent z.
-  induction H; intros.
-  - simpl. rewrite app_nil_r in H0. eauto.
-  - rewrite <- app_assoc.
-    apply multistep_step with y; auto. apply IHmultistep.
-    rewrite <- app_assoc; auto.
+  induction H; intros; eauto.
 Qed.
 
 Theorem multistep_R : forall α β (x y : tm),
     α ⊧ x ↪{ β } y -> α ⊧ x ↪*{ β } y.
-Proof. intros.
-  setoid_rewrite <- app_nil_r at 2. eauto.
+Proof. intros. eauto.
 Qed.
 
 Lemma multi_step_regular: forall α β e1 e2, α ⊧ e1 ↪*{ β } e2 -> lc e1 /\ lc e2.
@@ -134,7 +129,7 @@ Ltac step_regular_simp :=
     | [H: _ ⊧ _ ↪{ _ } _ |- body _] => apply step_regular in H; destruct H; auto
     end.
 
-Lemma value_reduction_refl: forall α β (v1: value) v2, α ⊧ v1 ↪*{ β} v2 -> v2 = v1 /\ β = [].
+Lemma value_reduction_refl: forall α β (v1: value) v2, α ⊧ v1 ↪*{ β} v2 -> v2 = v1 /\ β = α.
 Proof.
   intros * H.
   sinvert H; easy.
@@ -148,8 +143,8 @@ Ltac reduction_simp :=
 
 Lemma reduction_tlete:  forall e_x e α β (v : value),
     α ⊧ tlete e_x e ↪*{ β } v ->
-    (exists (βx βe: trace) (v_x: value),
-      β = βx ++ βe /\ α ⊧ e_x ↪*{ βx } v_x /\ (α ++ βx) ⊧ (e ^t^ v_x) ↪*{ βe } v).
+    (exists (βx: trace) (v_x: value),
+      α ⊧ e_x ↪*{ βx } v_x /\ βx ⊧ (e ^t^ v_x) ↪*{ β } v).
 Proof.
   intros.
   remember (tlete e_x e). remember (treturn v).
@@ -157,10 +152,7 @@ Proof.
   induction H; intros; subst. easy.
   sinvert H.
   - ospecialize* IHmultistep; eauto.
-    simp_hyps.
-    eexists _, _, _. split; [ | split ]; cycle 1.
-    econstructor; eauto. simplify_list_eq. eauto.
-    simplify_list_eq. eauto.
+    simp_hyps. repeat esplit; eauto.
   - repeat esplit. econstructor; eauto. eauto.
 Qed.
 
@@ -170,8 +162,8 @@ Lemma reduction_tlete':  forall e_x e α βx βe (v_x v : value),
     lemmas. *)
     body e ->
     α ⊧ e_x ↪*{ βx } v_x ->
-    (α ++ βx) ⊧ (e ^t^ v_x) ↪*{ βe } v ->
-    α ⊧ tlete e_x e ↪*{ βx ++ βe } v.
+    βx ⊧ (e ^t^ v_x) ↪*{ βe } v ->
+    α ⊧ tlete e_x e ↪*{ βe } v.
 Proof.
   intros * Hb H. remember (treturn v_x).
   induction H; intros; subst.
@@ -210,7 +202,6 @@ Proof.
   simpl. apply letapp_lc_body. repeat split; eauto using lc.
   by rewrite open_rec_lc_value.
   simpl. simplify_list_eq. rewrite open_rec_lc_value; eauto.
-  eauto.
 Qed.
 
 Lemma reduction_letapplam α Tb e (v_x : value) β (v : value) :
@@ -226,8 +217,7 @@ Proof.
   sinvert H1. sinvert H.
   apply reduction_tlete in H0.
   simp_hyps. simpl in *.
-  sinvert H2; try easy.
-  simplify_list_eq; eauto.
+  eapply multistep_trans; eauto.
 Qed.
 
 Lemma reduction_letapplam' α Tb e (v_x : value) β (v : value) :
@@ -252,14 +242,13 @@ Proof.
   rewrite open_rec_lc_value by eauto.
   simplify_list_eq. eapply reduction_tlete'; eauto.
   simpl. econstructor. eauto using multi_step_regular2.
-  simplify_list_eq. auto.
 Qed.
 
 Lemma reduction_tletapp:  forall v1 v2 e α β (v : value),
     α ⊧ tletapp v1 v2 e ↪*{ β} v ->
-    (exists (βx βe: trace) (v_x: value),
-      β = βx ++ βe /\ α ⊧ mk_app_e_v v1 v2 ↪*{ βx } v_x /\
-        (α ++ βx) ⊧ (e ^t^ v_x) ↪*{ βe } v).
+    (exists (βx: trace) (v_x: value),
+      α ⊧ mk_app_e_v v1 v2 ↪*{ βx } v_x /\
+        βx ⊧ (e ^t^ v_x) ↪*{ β } v).
 Proof.
   intros.
   remember (tletapp v1 v2 e). remember (treturn v).
@@ -269,11 +258,11 @@ Proof.
   simp_hyps. sinvert H.
   - eapply reduction_tlete in H0. simp_hyps.
     simplify_list_eq.
-    eexists _, _, _. split; [| split]; eauto using reduction_letapplam'.
+    eexists _, _. repeat split; eauto using reduction_letapplam'.
   - simplify_list_eq.
     ospecialize* H1; eauto. simp_hyps.
-    eexists _, _, _.
-    repeat split; cycle 1.
+    eexists _, _.
+    repeat split; cycle 1; eauto.
 
     (* Maybe this should be a lemma about [vfix]. *)
     apply reduction_mk_app_e_v in H.
@@ -282,16 +271,12 @@ Proof.
     simplify_list_eq. eauto.
     apply multi_step_regular1 in H0.
     sinvert H0. eauto.
-
-    simplify_list_eq. eauto.
-    simplify_list_eq. eauto.
 Qed.
 
 Lemma reduction_tleteffop:  forall op v2 e α β (v : value),
     α ⊧ (tleteffop op v2 e) ↪*{ β} v ->
-    exists (c2 c_x: constant) β',
-      v2 = c2 /\ β = ev{ op ~ c2 := c_x } :: β' /\
-        α ⊧{op ~ c2}⇓{ c_x } /\ (α ++ [ev{op ~ c2 := c_x}]) ⊧ (e ^t^ c_x) ↪*{ β'} v .
+    exists (c2 c_x: constant) βx,
+      v2 = c2 /\ α ⊧{op ~ c2}⇓{ βx }{ c_x } /\ βx ⊧ (e ^t^ c_x) ↪*{ β} v.
 Proof.
   intros.
   sinvert H. sinvert H0.
