RefinementType.v
@@ -26,27 +26,38 @@ Inductive rty : Type :=
 | rtyTd (ρ: rty) (td: transducer)
 | rtyArr (ρ: rty) (τ: rty).
 
-Fixpoint pure_rty (τ: rty) :=
-  match τ with
-  | rtyBase _ _ _ => True
-  | rtyTd _ _ => False
-  | rtyArr ρ1 ρ2 => pure_rty ρ1 /\ pure_rty ρ2
-  end.
-
-Fixpoint fine_rty (τ: rty) :=
-  match τ with
-  | rtyBase _ _ _ => True
-  | rtyTd ρ _ => pure_rty ρ
-  | rtyArr ρ τ => pure_rty ρ /\ fine_rty τ
-  end.
-
-Global Hint Constructors rty: core.
-
 Notation "'{:' b '|' ϕ '}'" := (rtyBase Over b ϕ) (at level 5, format "{: b | ϕ }", b constr, ϕ constr).
 Notation "'[:' b '|' ϕ ']'" := (rtyBase Under b ϕ) (at level 5, format "[: b | ϕ ]", b constr, ϕ constr).
 Notation "ρ '!<[' a ']>'" := (rtyTd ρ a) (at level 5, format "ρ !<[ a ]>", ρ constr, a constr).
 Notation "ρ '⇨' τ " :=
   (rtyArr ρ τ) (at level 80, format "ρ ⇨ τ", right associativity, ρ constr, τ constr).
+
+(** Over-Base type and function type is *pure*, which means it can be paramater of a function type; also can be introduced into type context *)
+Definition pure_rty (τ: rty) :=
+  match τ with
+  | rtyBase Over _ _ => True
+  | rtyBase Under _ _ => False
+  | rtyTd _ _ => False
+  | rtyArr ρ1 ρ2 => True
+  end.
+
+(** Fine-defined Refinement type:
+    - { b | ϕ }
+    - [ b | ϕ ] ! T
+    - (τ1 ⇨ τ2) ! T where τ1 ⇨ τ2 is fine-defined
+    - τ1 ⇨ τ2 where τ1 and τ2 is fine-defined, τ1 is pure
+ *)
+Fixpoint fine_rty (τ: rty) :=
+  match τ with
+  | rtyBase Over _ _ => True
+  | rtyBase Under _ _ => False
+  | rtyTd (rtyBase Under _ _) _ => True
+  | rtyTd (rtyArr ρ τ) _ => pure_rty ρ /\ fine_rty ρ /\ fine_rty τ
+  | rtyTd _ _ => False
+  | rtyArr ρ τ => pure_rty ρ /\ fine_rty ρ /\ fine_rty τ
+  end.
+
+Global Hint Constructors rty: core.
 
 (** Type erasure (Fig. 5) *)
 
@@ -80,7 +91,7 @@ Arguments rty_stale /.
 Fixpoint rty_open (k: nat) (s: value) (ρ: rty) : rty :=
   match ρ with
   | rtyBase ou b ϕ => rtyBase ou b (qualifier_open (S k) s ϕ)
-  | ρ !<[ a ]> => (rty_open k s ρ) !<[ td_open k s a ]>
+  | ρ !<[ a ]> => (rty_open k s ρ) !<[ td_open (S k) s a ]>
   | ρ ⇨ τ => (rty_open k s ρ) ⇨ (rty_open (S k) s τ)
   end.
 
@@ -97,14 +108,16 @@ Fixpoint rty_subst (k: atom) (s: value) (ρ: rty) : rty :=
 Notation "'{' x ':=' s '}r'" := (rty_subst x s) (at level 20, format "{ x := s }r", x constr).
 
 (** Local closure *)
-
+(** NOTE: all (L: aset) should be the first hypothesis *)
 Inductive lc_rty : rty -> Prop :=
 | lc_rtyBase: forall ou b ϕ, lc_phi1 ϕ -> fine_rty (rtyBase ou b ϕ) -> lc_rty (rtyBase ou b ϕ)
-| lc_rtyTd: forall ρ td, lc_rty ρ -> lc_td td -> fine_rty (rtyTd ρ td) -> lc_rty (rtyTd ρ td)
+| lc_rtyTd: forall ρ td (L : aset),
+    (forall x : atom, x ∉ L -> lc_td (td ^a^ x)) ->
+    fine_rty (rtyTd ρ td) -> lc_rty ρ ->
+    lc_rty (rtyTd ρ td)
 | lc_rtyArr: forall ρ τ (L : aset),
-    lc_rty ρ ->
     (forall x : atom, x ∉ L -> lc_rty (τ ^r^ x)) ->
-    fine_rty (ρ ⇨ τ) ->
+    fine_rty (ρ ⇨ τ) -> lc_rty ρ ->
     lc_rty (ρ ⇨ τ).
 
 Lemma lc_rty_fine: forall τ, lc_rty τ -> fine_rty τ.
@@ -117,12 +130,21 @@ Qed.
 Inductive closed_rty (d : aset) (ρ: rty): Prop :=
 | closed_rty_: lc_rty ρ -> rty_fv ρ ⊆ d -> closed_rty d ρ.
 
+Lemma closed_rty_fine: forall d τ, closed_rty d τ -> fine_rty τ.
+Proof.
+  pose lc_rty_fine.
+  induction 1; eauto.
+Qed.
+
 (** Well-formedness of type context. All terms and types are alpha-converted to
-  have unique names. *)
+  have unique names.
+  all rty in ctx are pure.
+ *)
 Inductive ok_ctx: listctx rty -> Prop :=
 | ok_ctx_nil: ok_ctx []
 | ok_ctx_cons: forall (Γ: listctx rty)(x: atom) (ρ: rty),
     ok_ctx Γ ->
+    pure_rty ρ ->
     closed_rty (ctxdom Γ) ρ ->
     x ∉ ctxdom Γ ->
     ok_ctx (Γ ++ [(x, ρ)]).
