Instantiation.v
@@ -4,6 +4,7 @@ From CT Require Import CoreLangProp.
 From CT Require Import OperationalSemantics.
 From CT Require Import BasicTypingProp.
 From CT Require Import Qualifier.
+From CT Require Import Transducer.
 From CT Require Import RefinementType.
 
 Import Atom.
@@ -13,6 +14,8 @@ Import NamelessTactics.
 Import OperationalSemantics.
 Import BasicTyping.
 Import Trace.
+Import Transducer.
+Import RefinementType.
 
 (** This file defines valuation environment, i.e., substitution (σ), and
   multi-substitution operation. *)
@@ -29,8 +32,7 @@ Definition msubst {A} (subst : atom -> value -> A -> A)
   map_fold subst a env.
 
 Notation "'m{' x '}q'" := (msubst qualifier_subst x) (at level 20, format "m{ x }q", x constr).
-Notation "'m{' x '}p'" := (msubst pty_subst x) (at level 20, format "m{ x }p", x constr).
-Notation "'m{' x '}a'" := (msubst am_subst x) (at level 20, format "m{ x }a", x constr).
-Notation "'m{' x '}h'" := (msubst hty_subst x) (at level 20, format "m{ x }h", x constr).
+Notation "'m{' x '}a'" := (msubst td_subst x) (at level 20, format "m{ x }a", x constr).
+Notation "'m{' x '}r'" := (msubst rty_subst x) (at level 20, format "m{ x }r", x constr).
 Notation "'m{' x '}v'" := (msubst value_subst x) (at level 20, format "m{ x }v", x constr).
 Notation "'m{' x '}t'" := (msubst tm_subst x) (at level 20, format "m{ x }t", x constr).
