TransducerProp.v
@@ -1,0 +1,154 @@
+From stdpp Require Import mapset.
+From stdpp Require Import natmap.
+From CT Require Import CoreLangProp.
+From CT Require Import OperationalSemantics.
+From CT Require Import BasicTypingProp.
+From CT Require Import Qualifier.
+From CT Require Import ListCtx.
+From CT Require Import Transducer.
+
+Import Atom.
+Import CoreLang.
+Import Tactics.
+Import NamelessTactics.
+Import OperationalSemantics.
+Import BasicTyping.
+Import Qualifier.
+Import ListCtx.
+Import List.
+Import Transducer.
+
+(** * Naming properties of refinement type syntax *)
+
+(** * subst *)
+
+Lemma subst_commute_td : forall x u_x y u_y a,
+    x <> y -> x ∉ fv_value u_y -> y ∉ fv_value u_x ->
+    {x := u_x }a ({y := u_y }a a) = {y := u_y }a ({x := u_x }a a).
+Proof.
+  pose subst_commute_value.
+  pose subst_commute_qualifier.
+  intros.
+  induction a; simpl; eauto; f_equal; eauto.
+Qed.
+
+Lemma subst_fresh_td: forall (a: transducer) (x:atom) (u: value),
+    x # a -> {x := u}a a = a.
+Proof.
+  pose subst_fresh_qualifier.
+  pose subst_fresh_value.
+  intros.
+  induction a; simpl in *; eauto; repeat f_equal;
+  try (auto_apply; my_set_solver).
+Qed.
+
+Lemma open_fv_td (a : transducer) (v : value): forall k,
+  td_fv ({k ~a> v} a) ⊆ td_fv a ∪ fv_value v.
+Proof.
+  pose open_fv_qualifier.
+  pose open_fv_value.
+  induction a; simpl; eauto; try my_set_solver.
+Qed.
+
+Lemma open_fv_td' (a : transducer) (v : value): forall k,
+  td_fv a ⊆ td_fv ({k ~a> v} a).
+Proof.
+  pose open_fv_qualifier'.
+  induction a; intros; simpl; eauto.
+Admitted.
+
+Lemma open_subst_same_td: forall x y (a : transducer) k,
+    x # a ->
+    {x := y }a ({k ~a> x} a) = {k ~a> y} a.
+Proof.
+  induction a; cbn; intros; eauto.
+  f_equal. eauto using open_subst_same_qualifier.
+  all:
+  repeat
+    match goal with
+    | H : forall k, _ # _ -> _ =_ |- _ => rewrite H by my_set_solver; eauto
+    end.
+Admitted.
+
+Lemma subst_open_td: forall (a: transducer) (x:atom) (u: value) (w: value) (k: nat),
+    lc w -> {x := w}a ({k ~a> u} a) = ({k ~a> {x := w}v u} ({x := w}a a)).
+Proof.
+  induction a; cbn; intros; eauto.
+  f_equal. eauto using subst_open_qualifier.
+  all:
+  repeat
+    match goal with
+    | H : context [lc _ -> _] |- _ => rewrite H by my_set_solver; eauto
+    end.
+Admitted.
+
+Lemma subst_open_td_closed:
+  ∀ (a : transducer) (x : atom) (u w : value) (k : nat),
+    closed_value u ->
+    lc w → {x := w }a ({k ~a> u} a) = {k ~a> u} ({x := w }a a).
+Proof.
+  intros. rewrite subst_open_td; auto.
+  rewrite (subst_fresh_value); eauto. set_solver.
+Qed.
+
+
+Lemma subst_open_var_td: forall x y (u: value) (a: transducer) (k: nat),
+    x <> y -> lc u -> {x := u}a ({k ~a> y} a) = ({k ~a> y} ({x := u}a a)).
+Proof.
+  intros.
+  rewrite subst_open_td; auto. simpl. rewrite decide_False; auto.
+Qed.
+
+
+Lemma subst_lc_td : forall x (u: value) (a: transducer),
+    lc_td a -> lc u -> lc_td ({x := u}a a).
+Proof.
+  pose subst_lc_phi1.
+  pose subst_lc_phi2.
+  pose subst_lc_value.
+  induction 1; intros Hu; eauto using lc_td.
+  - simpl. auto_exists_L. intros y Hy. specialize_with y.
+    rewrite subst_open_var_td in *; eauto. set_solver.
+Qed.
+
+Lemma fv_of_subst_td_closed:
+  forall x (u : value) (a: transducer),
+    closed_value u ->
+    td_fv ({x := u }a a) = (td_fv a ∖ {[x]}).
+Proof.
+  induction a; simpl; eauto using fv_of_subst_qualifier_closed.
+Admitted.
+
+Lemma open_not_in_eq_td (x : atom) (a : transducer) k :
+  x # {k ~a> x} a ->
+  forall e, a = {k ~a> e} a.
+Proof.
+  induction a; simpl; intros; eauto.
+  f_equal. eapply open_not_in_eq_qualifier. my_set_solver.
+  (* all: f_equal; auto_apply; my_set_solver. *)
+Admitted.
+
+Lemma lc_subst_td:
+  forall x (u: value) (a: transducer), lc_td ({x := u}a a) -> lc u -> lc_td a.
+Proof.
+  intros.
+  remember (({x:=u}a) a).
+  generalize dependent a.
+  induction H; intros;
+      match goal with
+      | H : _ = {_:=_}a ?a |- _ => destruct a; simpl in *; simplify_eq
+      end; eauto using lc_td.
+  econstructor.
+  (* auto_exists_L_intros. specialize_with x0. specialize_with y. *)
+  (* rewrite <- !subst_open_var_qualifier in H by (eauto; my_set_solver). *)
+  (* eauto using lc_subst_qualifier. *)
+Admitted.
+
+Lemma open_td_idemp: forall u (v: value) (a: transducer) (k: nat),
+    lc v ->
+    {k ~a> u} ({k ~a> v} a) = ({k ~a> v} a).
+Proof.
+  pose open_qualifier_idemp.
+  pose open_value_idemp.
+  induction a; intros; simpl; f_equal; eauto.
+Qed.
